Galois.v
@@ -303,15 +303,15 @@ Definition uco_sharp {A C : Set} (ϕ : @Uco C)
 (*  for relational properties       *)
 (************************************)
 
-Definition low_rel_prod  {A C : Set} (rel : C -> A -> Prop) : (C * C -> Prop) -> (A * A -> Prop) :=
+Definition low_rel_prod  {A C : Type} (rel : C -> A -> Prop) : (C * C -> Prop) -> (A * A -> Prop) :=
   fun c =>
     fun a : A * A => exists x : C * C, c x /\ rel (fst x) (fst a) /\ rel (snd x) (snd a).
 
-Definition up_rel_prod {A C : Set} (rel : C -> A -> Prop) : (A * A -> Prop) -> (C * C -> Prop) :=
+Definition up_rel_prod {A C : Type} (rel : C -> A -> Prop) : (A * A -> Prop) -> (C * C -> Prop) :=
   fun a =>
     fun c : C * C => forall y : A * A, rel (fst c) (fst y) -> rel (snd c) (snd y) -> a y.
 
-Lemma induced_adj_law_prod {A C : Set} (rel : C -> A -> Prop) :
+Lemma induced_adj_law_prod {A C : Type} (rel : C -> A -> Prop) :
   @Adjunction_law (A * A) (C * C) (low_rel_prod rel) (up_rel_prod rel).
 Proof.
   move => a c. rewrite /low_rel_prod /up_rel_prod. split.
@@ -321,7 +321,7 @@ Proof.
   + move => H x [y [c_y [rel_y_x_1 rel_y_x_2]]]. by apply: (H y).
 Qed.
 
-Definition induced_connection_prod {A C : Set} (rel : C -> A -> Prop)
+Definition induced_connection_prod {A C : Type} (rel : C -> A -> Prop)
   : Galois_Connection (A * A) (C * C) :=
   Build_Galois_Connection (induced_adj_law_prod rel).
 
