Robust2relSafetyProperty.v
@@ -1,0 +1,110 @@
+From mathcomp Require Import all_ssreflect.
+
+Set Implicit Arguments.
+Unset Printing Implicit Defensive.
+
+Require Import ClassicalExtras.
+Require Import MyNotation.
+Require Import Setoid.
+Require Import FunctionalExtensionality.
+
+Require Import Galois.
+Require Import LanguageModel.
+Require Import TraceModel.
+Require Import Properties.
+Require Import ChainModel.
+
+Require Import Robust2relTraceProperty. 
+
+Require Import PropExtensionality.
+Definition prop_extensionality := propositional_extensionality.
+
+Section Robust2relSafetyPreservation.
+
+  Variable Source Target: Language.
+  Variable compilation_chain : CompilationChain Source Target.
+
+  Variable T_evs S_evs : Events.
+  Variable T_end S_end : Endstates.
+
+  Locate Safety.
+
+  Local Definition trace__S := @trace S_evs S_end.
+  Local Definition finpref__S := @finpref S_evs S_end.
+  Local Definition trace__T := @trace T_evs T_end.
+  Local Definition finpref__T := @finpref T_evs T_end.
+
+  Local Definition prop__S := prop trace__S.
+  Local Definition Safety__S := @Safety S_evs S_end.
+  Local Definition prop__T := prop trace__T.
+  Local Definition Safety__T := @Safety T_evs T_end.
+
+  Variable Source_Semantics : Semantics Source trace__S.
+  Variable Target_Semantics : Semantics Target trace__T.
+
+  Local Definition sem__S := sem Source_Semantics.
+  Local Definition sem__T := sem Target_Semantics.
+  Local Definition par__S := par Source.
+  Local Definition par__T := par Target.
+  Local Definition ctx__S := ctx Source.
+  Local Definition ctx__T := ctx Target.
+  Local Definition rsat__S := rsat2 Source_Semantics.
+  Local Definition rsat__T := rsat2 Target_Semantics.
+
+  Local Definition cmp := compile_par Source Target compilation_chain.
+
+  Local Notation "P ↓" := (cmp P) (at level 50).
+ (* CA: don't understand why this does not work
+
+   Local Notation " C [ P ] " := (plug _  P C) (at level 50).
+  *)
+  Local Definition plug__S:= plug Source.
+  Local Definition plug__T := plug Target.
+
+  Variable σ : (trace__T * trace__T -> Prop) -> (trace__S * trace__S -> Prop).
+  Variable τ : (trace__S * trace__S -> Prop) -> (trace__T * trace__T -> Prop).
+
+  Definition σR2rP (P1 P2 : par__S) (π : trace__T * trace__T -> Prop) :=
+    rsat__S P1 P2 (σ π) -> rsat__T (P1 ↓) (P2 ↓) π.
+
+
+   Lemma contra_σR2rP (P1 P2 : par__S) (T : trace__T * trace__T -> Prop) :
+    (σR2rP P1 P2 T) <->  ((exists C__T t1 t2, sem__T ( plug__T (P1 ↓) C__T) t1 /\
+                                      sem__T ( plug__T (P2 ↓) C__T) t2 /\  ~ (T (t1,t2))) ->
+                        (exists C__S s1 s2, sem__S (plug__S P1 C__S) s1 /\
+                                      sem__S (plug__S P2 C__S) s2 /\
+                                    ~ (σ T) (s1, s2))).
+  Proof.
+    rewrite /σR2rP. by rewrite [_ -> _] contra !neg_rsat2.
+  Qed.
+
+  
+  Definition σR2rSP := forall P1 P2 π, Safety2 π -> σR2rP P1 P2 π.
+
+  Definition s2Cl_τR2rP (P1 P2 : par__S) (S : trace__S * trace__S -> Prop) :=
+    rsat__S P1 P2 S -> rsat__T (P1 ↓) (P2 ↓) ((s2Cl ∘ τ) S).
+
+  Definition s2Cl_τR2rTP := forall P1 P2 S, s2Cl_τR2rP P1 P2 S.
+
+  Theorem Adj_σR2rSP_iff_s2Cl_τR2rTP :
+    Adjunction_law τ σ -> (σR2rSP <-> s2Cl_τR2rTP).
+  Proof.
+    rewrite Galois_equiv. 
+    move => [mono1 [mono2 [G1 G2]]]. split.
+    - move => Hσ P1 P2 S Hrsat_src. apply: (Hσ P1 P2 ((s2Cl ∘ τ) S)).
+      apply: s2Cl_Safety2.
+      apply: rsat2_upper_closed. exact Hrsat_src.
+      apply: subset_trans.
+      { apply: G1. } 
+      apply: mono2.
+      by apply: s2Cl_bigger. 
+    - move => Hτ P1 P2 T Hrrsat_tgt Hsrc.
+      have H : rsat__T (P1 ↓) (P2 ↓) ((s2Cl ∘ τ) (σ T)) by apply: Hτ.
+      apply: rsat2_upper_closed. exact H.
+      have heq: s2Cl T = T by apply: s2Cl_id_on_Safety2. 
+      rewrite -heq.
+      apply: s2Cl_mono. rewrite heq. 
+      by apply: G2.
+  Qed.
+ 
+End Robust2relSafetyPreservation.
